Updated examples

tests/AddDelay.bpl
@@ -69,17 +69,17 @@ procedure Net#anon$3#entry#4()
   modifies C, R, M, St;
 {
   var ActionPH#y: int;
-  assume C[Net#a] == 1;
-  assume C[Net#b] == 0;
-  assume C[Net#c] == 0;
-  assume C[Net#d] == 0;
+  assume C#init[Net#a] == 1;
+  assume C#init[Net#b] == 0;
+  assume C#init[Net#c] == 0;
+  assume C#init[Net#d] == 0;
   assume R[Net#a] == 0;
   assume R[Net#b] == 0;
   assume R[Net#c] == 0;
   assume R[Net#d] == 0;
+  assume C#init == C;
   C[Net#b] := C[Net#b] + 1;
   assume (M[Net#b][R[Net#b]] == M[Net#c][R[Net#c] - 1]) || (M[Net#b][R[Net#b]] == 0);
-  assume C#init == C;
   assert {:msg "  Channel invariant might not hold on action entry (generated #0)"} 0 <= R[Net#a];
   assert {:msg "  Channel invariant might not hold on action entry (generated #1)"} 0 <= C[Net#a];
   assert {:msg "  Channel invariant might not hold on action entry (generated #2)"} (R[Net#a] + C[Net#a]) == C#init[Net#a];
@@ -109,13 +109,14 @@ procedure Net#anon$3#entry#4()
 procedure Net#anon$3#Add#anon$0#5()
   modifies C, R, M, St;
 {
+  var ActionPH#y: int;
   var St#next: State;
   var in1#i: int;
   var in2#j: int;
-  assume C[Net#a] == 1;
-  assume C[Net#b] == 0;
-  assume C[Net#c] == 0;
-  assume C[Net#d] == 0;
+  assume C#init[Net#a] == 1;
+  assume C#init[Net#b] == 0;
+  assume C#init[Net#c] == 0;
+  assume C#init[Net#d] == 0;
   assume 0 <= R[Net#a];
   assume 0 <= C[Net#a];
   assume (R[Net#a] + C[Net#a]) == C#init[Net#a];
@@ -182,14 +183,15 @@ procedure Net#anon$3#Add#anon$0#5()
 procedure Net#anon$3#Delay#anon$2#6()
   modifies C, R, M, St;
 {
+  var ActionPH#y: int;
   var ActorParam#k: int;
   var St#next: State;
   var in#i: int;
   assume ActorParam#k == 0;
-  assume C[Net#a] == 1;
-  assume C[Net#b] == 0;
-  assume C[Net#c] == 0;
-  assume C[Net#d] == 0;
+  assume C#init[Net#a] == 1;
+  assume C#init[Net#b] == 0;
+  assume C#init[Net#c] == 0;
+  assume C#init[Net#d] == 0;
   assume 0 <= R[Net#a];
   assume 0 <= C[Net#a];
   assume (R[Net#a] + C[Net#a]) == C#init[Net#a];
@@ -252,10 +254,10 @@ procedure Net#anon$3#exit#7()
   modifies C, R, M, St;
 {
   var ActionPH#y: int;
-  assume C[Net#a] == 1;
-  assume C[Net#b] == 0;
-  assume C[Net#c] == 0;
-  assume C[Net#d] == 0;
+  assume C#init[Net#a] == 1;
+  assume C#init[Net#b] == 0;
+  assume C#init[Net#c] == 0;
+  assume C#init[Net#d] == 0;
   assume 0 <= R[Net#a];
   assume 0 <= C[Net#a];
   assume (R[Net#a] + C[Net#a]) == C#init[Net#a];
@@ -282,14 +284,14 @@ procedure Net#anon$3#exit#7()
   );
   assume (M[Net#b][0] == M[Net#c][-1]) || (M[Net#b][0] == 0);
   assume !(((1 <= C[Net#a]) && (1 <= C[Net#b])) || (1 <= C[Net#d]));
-  assert {:msg "  14.3: The network might leave unread tokens on channel a"} C[Net#a] == 0;
-  assert {:msg "  14.3: The network might leave unread tokens on channel b"} C[Net#b] == 0;
-  assert {:msg "  14.3: The network might not produce the specified number of tokens on output out"} C[Net#c] == 1;
-  assert {:msg "  14.3: The network might leave unread tokens on channel d"} C[Net#d] == 0;
   ActionPH#y := M[Net#c][0];
   assert {:msg "  15.13: Network action postcondition might not hold"} (ActionPH#y == (M[Net#c][R[Net#c] - 1] + M[Net#a][0])) || (ActionPH#y == M[Net#a][0]);
   R[Net#c] := R[Net#c] + C[Net#c];
-  C[Net#c] := 0;
+  C[Net#c] := C[Net#c] - 1;
   C[Net#b] := C[Net#b] - 1;
   assert {:msg "  19.13: The network might not preserve the network invariant"} (M[Net#b][R[Net#b]] == M[Net#c][R[Net#c] - 1]) || (M[Net#b][R[Net#b]] == 0);
+  assert {:msg "  14.3: The network might leave unread tokens on channel a"} C[Net#a] == 0;
+  assert {:msg "  14.3: The network might leave unread tokens on channel b"} C[Net#b] == 0;
+  assert {:msg "  14.3: The network might not produce the specified number of tokens on output out"} C[Net#c] == 0;
+  assert {:msg "  14.3: The network might leave unread tokens on channel d"} C[Net#d] == 0;
 }
